Lemmas.v
@@ -4,6 +4,7 @@ Open Scope list_scope.
 
 Module LemmasFn (Import G : Grammar.T).
   
+  (* Utility lemma: If a key-value pair exists in a map (find returns Some), then that key is in the map *)
   Lemma find_In : forall k vT (v : vT) m,
       NtMap.find k m = Some v ->
       NtMap.In k m.
@@ -12,6 +13,7 @@ Module LemmasFn (Import G : Grammar.T).
     unfold not. intro Hcontra. inv Hcontra.
   Qed.
   
+  (* Alias of find_In specifically for nonterminal maps - helps with readability *)
   Lemma ntmap_find_in : forall k vT (v : vT) m,
       NtMap.find k m = Some v ->
       NtMap.In k m.
@@ -20,12 +22,14 @@ Module LemmasFn (Import G : Grammar.T).
     unfold not. intro Hcontra. inv Hcontra.
   Qed.
   
+  (* Utility tactic to copy a hypothesis and apply find_In to it *)
   Ltac copy_and_find_In H :=
     let Hfind := fresh "Hfind" in
     let Heq   := fresh "Heq" in 
     remember H as Hfind eqn:Heq; clear Heq;
     apply find_In in H.
   
+  (* Proves that if all symbols in a list are nonterminals (isNT), then no terminal can be in that list *)
   Lemma T_not_in_NT_list :
     forall (gamma : list symbol) (y : terminal),
       forallb isNT gamma = true ->
@@ -41,7 +45,7 @@ Module LemmasFn (Import G : Grammar.T).
         apply H1. apply H0.
   Qed.
   
-  (* Some useful lemmas to remember : in_eq, in_cons *)
+  (* Shows that a list of all nonterminals cannot be equal to a list containing a terminal *)
   Lemma NT_list_neq_list_with_T :
     forall (gamma prefix suffix : list symbol)
            (y : terminal),
@@ -55,6 +59,7 @@ Module LemmasFn (Import G : Grammar.T).
     right. apply in_eq.
   Qed.
   
+  (* Proves that if all symbols in a list are terminals (isT), then no nonterminal can be in that list *)
   Lemma NT_not_in_T_list :
     forall (gamma : list symbol) (X : nonterminal),
       forallb isT gamma = true ->
@@ -70,6 +75,7 @@ Module LemmasFn (Import G : Grammar.T).
         apply H1. assumption.
   Qed.
   
+  (* Shows that a list of all terminals cannot be equal to a list containing a nonterminal *)
   Lemma T_list_neq_list_with_NT :
     forall (gamma prefix suffix : list symbol)
            (X : nonterminal),
@@ -83,279 +89,291 @@ Module LemmasFn (Import G : Grammar.T).
     right. apply in_eq.
   Qed.
 
+  (* Proves that if a key-value pair exists in the parse table (find returns Some), then that key is in the table *)
   Lemma pt_find_in :
-  forall k A (v : A) m,
-    ParseTable.find k m = Some v
-    -> ParseTable.In k m.
-Proof.
-  intros.
-  rewrite ParseTableFacts.in_find_iff.
-  rewrite H; congruence.
-Qed.
+    forall k A (v : A) m,
+      ParseTable.find k m = Some v
+      -> ParseTable.In k m.
+  Proof.
+    intros.
+    rewrite ParseTableFacts.in_find_iff.
+    rewrite H; congruence.
+  Qed.
 
-(*
-Lemma lookaheadmap_find_in : forall k vT (v : vT) m,
-    LaMap.find k m = Some v ->
-    LaMap.In k m.
-Proof.
-  intros. rewrite LaMapFacts.in_find_iff. rewrite H.
-  unfold not. intro Hcontra. inv Hcontra.
-Qed.
-*)
-Lemma pt_lookup_in :
-  forall x la tbl gamma,
-    pt_lookup x la tbl = Some gamma
-    -> ParseTable.In (x, la) tbl.
-Proof.
-  intros x la tbl gamma Hlkp.
-  unfold pt_lookup in Hlkp.
-  apply ParseTableFacts.in_find_iff; congruence.
-Qed.
+  (* Proves that if a lookup in the parse table succeeds, then the key exists in the table *)
+  Lemma pt_lookup_in :
+    forall x la tbl gamma,
+      pt_lookup x la tbl = Some gamma
+      -> ParseTable.In (x, la) tbl.
+  Proof.
+    intros x la tbl gamma Hlkp.
+    unfold pt_lookup in Hlkp.
+    apply ParseTableFacts.in_find_iff; congruence.
+  Qed.
 
-Lemma eof_first_sym :
-  forall g la sym,
-    first_sym g la sym
-    -> la = EOF
-    -> False.
-Proof.
-  induction 1; intros; auto.
-  inv H.
-Qed.
-
-Lemma eof_first_gamma :
-  forall g la gamma,
-    first_gamma g la gamma
-    -> la = EOF
-    -> False.
-Proof.
-  intros.
-  inv H.
-  eapply eof_first_sym; eauto.
-Qed.
-
-Lemma nullable_middle_sym :
-  forall g xs ys sym,
-    nullable_gamma g (xs ++ sym :: ys)
-    -> nullable_sym g sym.
-Proof.
-  induction xs; intros.
-  - simpl in H.
-    inv H.
-    auto.
-  - eapply IHxs.
-    inv H.
-    eauto.
-Qed.
-
-Lemma gamma_with_terminal_not_nullable :
-  forall g gpre y gsuf,
-    ~ nullable_gamma g (gpre ++ T y :: gsuf).
-Proof.
-  unfold not.
-  induction gpre as [| sym syms]; intros y gsuf Hnu; simpl in *.
-  - inv Hnu.
-    inv H1.
-  - destruct sym.
-    + inv Hnu.
-      inv H1.
-    + inv Hnu.
-      eapply IHsyms; eauto.
-Qed.
-
-Lemma nullable_split :
-  forall g xs ys,
-    nullable_gamma g (xs ++ ys)
-    -> nullable_gamma g ys.
-Proof.
-  induction xs; intros.
-  - auto.
-  - inv H.
-    eapply IHxs; eauto.
-Qed.
-
-(* New version, without mutual induction *)
-Lemma no_first_follow_conflicts :
-  forall tbl g,
-    parse_table_correct tbl g
-    -> forall la sym,
+  (* Proves that EOF cannot be a first symbol of any symbol in the grammar *)
+  Lemma eof_first_sym :
+    forall g la sym,
       first_sym g la sym
-      -> nullable_sym g sym
-      -> follow_sym g la sym
+      -> la = EOF
       -> False.
-Proof.
-  intros tbl g Htbl la sym Hfi.
-  induction Hfi; intros.
-  - inv H.
-  - inv H1.
-    assert (ys = gpre ++ s :: gsuf).
-    { destruct Htbl as [Hmin Hcom].
-      assert (Hlk : lookahead_for la x (gpre ++ s :: gsuf) g).
-      { unfold lookahead_for; auto. }
-      assert (Hlk' : lookahead_for la x ys g).
-      { unfold lookahead_for; auto. }
-      unfold pt_complete in Hcom.
-      eapply Hcom in Hlk; eauto.
-      eapply Hcom in Hlk'; eauto.
-      congruence. }
-    subst.
-    eapply IHHfi.
-    + apply nullable_middle_sym in H5; auto.
-    + destruct s.
-      * apply gamma_with_terminal_not_nullable in H5; inv H5.
-      * eapply FollowLeft; eauto.
-        assert (NT n :: gsuf = [NT n] ++ gsuf) by auto.
-        rewrite H1 in H5.
-        rewrite app_assoc in H5.
-        apply nullable_split in H5.
-        auto.
-Qed.
+  Proof.
+    induction 1; intros; auto.
+    inv H.
+  Qed.
 
-Lemma sym_derives_nil_nullable :
-  forall g sym wpre f wsuf,
-    sym_derives_prefix g sym wpre f wsuf
-    -> wpre = nil
-    -> nullable_sym g sym.
-Proof.
-  intros g sym wpre f wsuf Hder.
-  induction Hder using sdp_mutual_ind with
-      (P := fun sym wpre tr wsuf
-                (pf : sym_derives_prefix g sym wpre tr wsuf) =>
-              wpre = nil
-              -> nullable_sym g sym)
-      (P0 := fun gamma wpre f wsuf
-                 (pf : gamma_derives_prefix g gamma wpre f wsuf)
-             =>
-               wpre = nil
-               -> nullable_gamma g gamma); intros; subst.
-  - inv H.
-  - simpl in *.
-    econstructor; eauto.
-  - constructor.
-  - apply app_eq_nil in H; destruct H; subst.
-    destruct IHHder; auto.
-    constructor; auto.
-    econstructor; eauto.
-Qed.
+  (* Proves that EOF cannot be a first symbol of any sequence of symbols in the grammar *)
+  Lemma eof_first_gamma :
+    forall g la gamma,
+      first_gamma g la gamma
+      -> la = EOF
+      -> False.
+  Proof.
+    intros.
+    inv H.
+    eapply eof_first_sym; eauto.
+  Qed.
 
-Lemma gamma_derives_cons_first_gamma :
-  forall g gamma word f rem,
-    gamma_derives_prefix g gamma word f rem
-    -> forall t v toks,
-      word = (existT _ t v) :: toks
-      -> first_gamma g (LA t) gamma.
-Proof.
-  intros g gamma word f rem Hder.
-  induction Hder using gdp_mutual_ind with
-      (P := fun sym word tr rem
-                (pf : sym_derives_prefix g sym word tr rem) =>
-              forall t v toks,
-                word = (existT _ t v) :: toks
-                -> first_sym g (LA t) sym)
-      (P0 := fun gamma word f rem
-                 (pf : gamma_derives_prefix g gamma word f rem)
-             =>
-               forall t v toks,
-                 word = (existT _ t v) :: toks
-                 -> first_gamma g (LA t) gamma); intros; subst.
-  - inv H; constructor.
-  - simpl in *.
-    specialize (IHHder t v toks).
-    destruct IHHder; auto.
-    econstructor; eauto.
-  - inv H.
-  - destruct s.
-    + inv s0.
+  (* If a sequence of symbols is nullable and contains a symbol in the middle, that symbol must be nullable *)
+  Lemma nullable_middle_sym :
+    forall g xs ys sym,
+      nullable_gamma g (xs ++ sym :: ys)
+      -> nullable_sym g sym.
+  Proof.
+    induction xs; intros.
+    - simpl in H.
       inv H.
-      eapply FirstGamma with (gpre := nil); constructor.
-    + destruct wpre as [| ptok ptoks]; simpl in *.
-      * subst.
-        specialize (IHHder0 t v0 toks).
-        destruct IHHder0; auto.
-        eapply FirstGamma with (gpre := NT n :: gpre).
-        -- constructor; auto.
-           apply sym_derives_nil_nullable in s0; auto.
-        -- auto.
-      * inv H.
-        eapply FirstGamma with (gpre := nil).
-        -- constructor.
-        -- eapply IHHder; eauto.
-Qed.
+      auto.
+    - eapply IHxs.
+      inv H.
+      eauto.
+  Qed.
 
-Lemma tbl_entry_is_lookahead :
-  forall tbl g x x' la gamma f,
-    parse_table_correct tbl g
-    -> pt_lookup x la tbl = Some (existT _ (x', gamma) f)
-    -> lookahead_for la x gamma g.
-Proof.
-  intros tbl g x x' la gamma f Htbl Hlkp.
-  destruct Htbl as [Hsou Hcom].
-  unfold pt_sound in Hsou.
-  apply Hsou in Hlkp; destruct Hlkp as [Heq [Hin Hl]]; subst; auto.
-Qed.
+  (* A sequence containing a terminal symbol cannot be nullable *)
+  Lemma gamma_with_terminal_not_nullable :
+    forall g gpre y gsuf,
+      ~ nullable_gamma g (gpre ++ T y :: gsuf).
+  Proof.
+    unfold not.
+    induction gpre as [| sym syms]; intros y gsuf Hnu; simpl in *.
+    - inv Hnu.
+      inv H1.
+    - destruct sym.
+      + inv Hnu.
+        inv H1.
+      + inv Hnu.
+        eapply IHsyms; eauto.
+  Qed.
 
-Lemma first_gamma_first_sym :
-  forall g x la gamma f,
-    In (existT _ (x, gamma) f) g.(prods)
-    -> first_gamma g la gamma
-    -> first_sym g la (NT x).
-Proof.
-  intros g x la gamma f Hin Hfg.
-  inv Hfg.
-  econstructor; eauto.
-Qed.
+  (* If a concatenation of sequences is nullable, the suffix must be nullable *)
+  Lemma nullable_split :
+    forall g xs ys,
+      nullable_gamma g (xs ++ ys)
+      -> nullable_gamma g ys.
+  Proof.
+    induction xs; intros.
+    - auto.
+    - inv H.
+      eapply IHxs; eauto.
+  Qed.
 
-Lemma in_A_not_in_B_in_diff :
-  forall elt a b,
-    NtSet.In elt a
-    -> ~ NtSet.In elt b
-    -> NtSet.In elt (NtSet.diff a b).
-Proof.
-  ND.fsetdec.
-Defined.
+  (* Key property of LL(1) grammars: A symbol cannot have the same token in both its FIRST and FOLLOW sets if it's nullable *)
+  (* Or else, if symbol A is nullable and has token t in both FIRST(A) and FOLLOW(A), there is ambiguity:
+     When seeing token t, the parser wouldn't know whether to
+     1. Derive A to produce t
+     2. Skip A and use t as a lookahead for what comes after A
+  *)
+  Lemma no_first_follow_conflicts :
+    forall tbl g,
+      parse_table_correct tbl g
+      -> forall la sym,
+        first_sym g la sym
+        -> nullable_sym g sym
+        -> follow_sym g la sym
+        -> False.
+  Proof.
+    intros tbl g Htbl la sym Hfi.
+    induction Hfi; intros.
+    - inv H.
+    - inv H1.
+      assert (ys = gpre ++ s :: gsuf).
+      { destruct Htbl as [Hmin Hcom].
+        assert (Hlk : lookahead_for la x (gpre ++ s :: gsuf) g).
+        { unfold lookahead_for; auto. }
+        assert (Hlk' : lookahead_for la x ys g).
+        { unfold lookahead_for; auto. }
+        unfold pt_complete in Hcom.
+        eapply Hcom in Hlk; eauto.
+        eapply Hcom in Hlk'; eauto.
+        congruence. }
+      subst.
+      eapply IHHfi.
+      + apply nullable_middle_sym in H5; auto.
+      + destruct s.
+        * apply gamma_with_terminal_not_nullable in H5; inv H5.
+        * eapply FollowLeft; eauto.
+          assert (NT n :: gsuf = [NT n] ++ gsuf) by auto.
+          rewrite H1 in H5.
+          rewrite app_assoc in H5.
+          apply nullable_split in H5.
+          auto.
+  Qed.
 
-Lemma in_list_iff_in_fromNtList :
-  forall x l, In x l <-> NtSet.In x (fromNtList l).
-Proof.
-  split; intros; induction l; simpl in *.
-  - inv H.
-  - destruct H; subst; auto.
-    + ND.fsetdec.
-    + apply IHl in H; ND.fsetdec.
-  - ND.fsetdec.
-  - destruct (NtSetFacts.eq_dec x a); subst; auto.
-    right. apply IHl. ND.fsetdec.
-Defined.
+  (* If a symbol derives an empty prefix, then that symbol must be nullable *)
+  Lemma sym_derives_nil_nullable :
+    forall g sym wpre f wsuf,
+      sym_derives_prefix g sym wpre f wsuf
+      -> wpre = nil
+      -> nullable_sym g sym.
+  Proof.
+    intros g sym wpre f wsuf Hder.
+    induction Hder using sdp_mutual_ind with
+        (P := fun sym wpre tr wsuf
+                  (pf : sym_derives_prefix g sym wpre tr wsuf) =>
+                wpre = nil
+                -> nullable_sym g sym)
+        (P0 := fun gamma wpre f wsuf
+                   (pf : gamma_derives_prefix g gamma wpre f wsuf)
+               =>
+                 wpre = nil
+                 -> nullable_gamma g gamma); intros; subst.
+    - inv H.
+    - simpl in *.
+      econstructor; eauto.
+    - constructor.
+    - apply app_eq_nil in H; destruct H; subst.
+      destruct IHHder; auto.
+      constructor; auto.
+      econstructor; eauto.
+  Qed.
 
-Lemma pt_lookup_elements' :
-  forall (k : ParseTable.key) (A : Type) (a : A) (l : list (ParseTable.key * A)),
-    findA (ParseTableFacts.eqb k) l = Some a
-    -> In (k, a) l.
-Proof.
-  intros k A a l Hf.
-  induction l as [| p l' IHl].
-  - inv Hf.
-  - simpl in *.
-    destruct p as (k', gamma').
-    destruct (ParseTableFacts.eqb k k') eqn:Heq.
-    + inv Hf.
-      unfold ParseTableFacts.eqb in *.
-      destruct (ParseTableFacts.eq_dec k k').
-      * subst; auto.
-      * inv Heq.
-    + right; auto.
-Defined.
+  (* If a sequence derives a token sequence starting with token t, then t must be in the FIRST set of that sequence *)
+  Lemma gamma_derives_cons_first_gamma :
+    forall g gamma word f rem,
+      gamma_derives_prefix g gamma word f rem
+      -> forall t v toks,
+        word = (existT _ t v) :: toks
+        -> first_gamma g (LA t) gamma.
+  Proof.
+    intros g gamma word f rem Hder.
+    induction Hder using gdp_mutual_ind with
+        (P := fun sym word tr rem
+                  (pf : sym_derives_prefix g sym word tr rem) =>
+                forall t v toks,
+                  word = (existT _ t v) :: toks
+                  -> first_sym g (LA t) sym)
+        (P0 := fun gamma word f rem
+                   (pf : gamma_derives_prefix g gamma word f rem)
+               =>
+                 forall t v toks,
+                   word = (existT _ t v) :: toks
+                   -> first_gamma g (LA t) gamma); intros; subst.
+    - inv H; constructor.
+    - simpl in *.
+      specialize (IHHder t v toks).
+      destruct IHHder; auto.
+      econstructor; eauto.
+    - inv H.
+    - destruct s.
+      + inv s0.
+        inv H.
+        eapply FirstGamma with (gpre := nil); constructor.
+      + destruct wpre as [| ptok ptoks]; simpl in *.
+        * subst.
+          specialize (IHHder0 t v0 toks).
+          destruct IHHder0; auto.
+          eapply FirstGamma with (gpre := NT n :: gpre).
+          -- constructor; auto.
+             apply sym_derives_nil_nullable in s0; auto.
+          -- auto.
+        * inv H.
+          eapply FirstGamma with (gpre := nil).
+          -- constructor.
+          -- eapply IHHder; eauto.
+  Qed.
+
+  (* If a parse table entry exists, it must correspond to a valid lookahead for that production *)
+  Lemma tbl_entry_is_lookahead :
+    forall tbl g x x' la gamma f,
+      parse_table_correct tbl g
+      -> pt_lookup x la tbl = Some (existT _ (x', gamma) f)
+      -> lookahead_for la x gamma g.
+  Proof.
+    intros tbl g x x' la gamma f Htbl Hlkp.
+    destruct Htbl as [Hsou Hcom].
+    unfold pt_sound in Hsou.
+    apply Hsou in Hlkp; destruct Hlkp as [Heq [Hin Hl]]; subst; auto.
+  Qed.
+
+  (* If a production exists in the grammar and its RHS has a token in its FIRST set, then that token is in the FIRST set of the LHS nonterminal *)
+  Lemma first_gamma_first_sym :
+    forall g x la gamma f,
+      In (existT _ (x, gamma) f) g.(prods)
+      -> first_gamma g la gamma
+      -> first_sym g la (NT x).
+  Proof.
+    intros g x la gamma f Hin Hfg.
+    inv Hfg.
+    econstructor; eauto.
+  Qed.
+
+  (* Set theory helper: If an element is in set A but not in set B, it must be in the difference A - B *)
+  Lemma in_A_not_in_B_in_diff :
+    forall elt a b,
+      NtSet.In elt a
+      -> ~ NtSet.In elt b
+      -> NtSet.In elt (NtSet.diff a b).
+  Proof.
+    ND.fsetdec.
+  Defined.
+
+  (* Equivalence between list membership and set membership for nonterminal lists *)
+  Lemma in_list_iff_in_fromNtList :
+    forall x l, In x l <-> NtSet.In x (fromNtList l).
+  Proof.
+    split; intros; induction l; simpl in *.
+    - inv H.
+    - destruct H; subst; auto.
+      + ND.fsetdec.
+      + apply IHl in H; ND.fsetdec.
+    - ND.fsetdec.
+    - destruct (NtSetFacts.eq_dec x a); subst; auto.
+      right. apply IHl. ND.fsetdec.
+  Defined.
+
+  (* Helper lemma for proving properties about parse table lookups using the elements representation *)
+  Lemma pt_lookup_elements' :
+    forall (k : ParseTable.key) (A : Type) (a : A) (l : list (ParseTable.key * A)),
+      findA (ParseTableFacts.eqb k) l = Some a
+      -> In (k, a) l.
+  Proof.
+    intros k A a l Hf.
+    induction l as [| p l' IHl].
+    - inv Hf.
+    - simpl in *.
+      destruct p as (k', gamma').
+      destruct (ParseTableFacts.eqb k k') eqn:Heq.
+      + inv Hf.
+        unfold ParseTableFacts.eqb in *.
+        destruct (ParseTableFacts.eq_dec k k').
+        * subst; auto.
+        * inv Heq.
+      + right; auto.
+  Defined.
       
-Lemma pt_lookup_elements :
-  forall x la tbl p,
-    pt_lookup x la tbl = Some p
-    -> In ((x, la), p) (ParseTable.elements tbl).
-Proof.
-  intros.
-  unfold pt_lookup in *.
-  rewrite ParseTableFacts.elements_o in H.
-  apply pt_lookup_elements'; auto.
-Defined.
+  (* Proves that successful parse table lookups correspond to elements in the table's list representation *)
+  Lemma pt_lookup_elements :
+    forall x la tbl p,
+      pt_lookup x la tbl = Some p
+      -> In ((x, la), p) (ParseTable.elements tbl).
+  Proof.
+    intros.
+    unfold pt_lookup in *.
+    rewrite ParseTableFacts.elements_o in H.
+    apply pt_lookup_elements'; auto.
+  Defined.
 
+  (* List operation helper: Shows that cons is equivalent to singleton append *)
   Lemma cons_app_singleton :
     forall A (x : A) (ys : list A),
       x :: ys = [x] ++ ys.
@@ -363,6 +381,7 @@ Defined.
     auto.
   Defined.
 
+  (* List operation helper: Shows that an element appears in a list that contains it *)
   Lemma in_app_cons :
     forall A (x : A) (pre suf : list A),
       In x (pre ++ x :: suf).
@@ -371,8 +390,7 @@ Defined.
     induction pre; simpl; auto.
   Defined.
 
-  (* alternative FirstGamma definition that simplifies
-     reasoning in some cases *)
+  (* Alternative inductive definition of first_gamma that is sometimes easier to work with *)
   Inductive first_gamma' (g : grammar) (la : lookahead) :
     list symbol -> Prop :=
   | FG_hd : forall h t,
@@ -383,6 +401,7 @@ Defined.
       -> first_gamma' g la t
       -> first_gamma' g la (h :: t).
 
+  (* Proves equivalence between the two definitions of first_gamma *)
   Lemma first_gamma_iff_first_gamma' :
     forall g la gamma,
       first_gamma g la gamma <-> first_gamma' g la gamma.
@@ -405,6 +424,8 @@ Defined.
                               (gsuf := gsuf); auto.
   Qed.
 
+  (* Helper lemma about list equality: If two lists with a common element in the middle are equal, 
+     either the element appears in the prefix of the other list, or the prefixes and suffixes are equal *)
   Lemma medial :
     forall A pre pre' (sym sym' : A) suf suf',
       pre ++ sym :: suf = pre' ++ sym' :: suf'
@@ -422,6 +443,7 @@ Defined.
         repeat destruct H; auto.
   Qed.
 
+  (* If a sequence is nullable and contains a symbol, that symbol must be nullable *)
   Lemma nullable_sym_in :
     forall g sym gamma,
       nullable_gamma g gamma
@@ -435,6 +457,8 @@ Defined.
       inv H0; auto.
   Qed.
 
+  (* If a sequence has a token in its FIRST set and is preceded by a nullable sequence,
+     the token is in the FIRST set of the concatenation *)
   Lemma first_gamma_split :
     forall g la xs ys,
       first_gamma g la ys
@@ -448,6 +472,7 @@ Defined.
     apply first_gamma_iff_first_gamma'; auto.
   Qed.
 
+  (* Technical lemma about associativity of list append under semantic type computation *)
   Lemma app_assoc_under_rhs_semty :
     forall xs ys zs,
       rhs_semty (xs ++ ys ++ zs) = rhs_semty ((xs ++ ys) ++ zs).
@@ -457,6 +482,7 @@ Defined.
     rewrite IHxs; auto.
   Qed.
 
+  (* If a production exists with a given RHS, another production must exist with an equal RHS *)
   Lemma rhss_eq_exists_prod' :
     forall g x gamma gamma' f,
       In (existT action_ty (x, gamma) f) g.(prods)
@@ -467,6 +493,8 @@ Defined.
     intros; simpl in *; subst; eauto.
   Qed.
 
+  (* If a symbol appears in a nullable prefix of a production and the suffix has a token in its FIRST set,
+     that token is in the FOLLOW set of the symbol *)
   Lemma follow_pre :
     forall g x la sym suf pre f,
       In (existT _ (x, pre ++ suf) f) g.(prods)
@@ -493,6 +521,8 @@ Defined.
       + rewrite <- app_assoc; auto.
   Qed.
 
+  (* Key property of LL(1) grammars: If two productions for the same nonterminal can derive the same first token,
+     they must be the same production *)
   Lemma first_sym_rhs_eqs :
     forall g t,
       parse_table_correct t g
@@ -525,6 +555,7 @@ Defined.
         apply FirstGamma with (gpre := []); auto.
   Qed.
 
+  (* If two lookups in a parse table succeed with the same key, they must return the same value *)
   Lemma lookups_eq :
     forall x la t xp xp',
       pt_lookup x la t = Some xp
@@ -534,6 +565,7 @@ Defined.
     intros; tc.
   Qed.
 
+  (* Decidability of equality for base productions *)
   Lemma base_production_eq_dec :
     forall (b b' : base_production),
       {b = b'} + {b <> b'}.
@@ -541,6 +573,7 @@ Defined.
     repeat decide equality.
   Defined.
 
+  (* If a production is in the grammar's production list, its base production is in the baseProductions list *)
   Lemma in_productions_in_baseProductions :
     forall g b f,
       In (existT _ b f) g.(prods)
@@ -551,6 +584,7 @@ Defined.
     induction g.(prods) as [| p ps]; simpl in *; inv Hin; auto.
   Qed.
 
+  (* If a base production is in the baseProductions list, there exists a production in the grammar's production list with that base *)
   Lemma in_baseProductions_exists_in_productions :
     forall g b,
       In b (baseProductions g)
