MyExample.v
@@ -1,0 +1,181 @@
+Require Import String.
+Require Import Grammar.
+Require Import Main.
+Require Import Generator.
+Open Scope string_scope.
+
+
+Inductive fact : Type :=
+  | num_fact : nat -> fact
+  | exp_fact : exp -> fact
+with term' : Type :=
+  | empty_term' : term'
+  | comb_term' : fact -> term' -> term'
+with term : Type :=
+  | comb_term : fact -> term' -> term
+with exp' : Type :=
+  | comb_exp' : term -> exp' -> exp'
+  | empty_exp' : exp'
+with exp : Type :=
+  | comb_exp : term -> exp' -> exp.
+
+(* First, we provide the types of grammar symbols 
+   and their decidable equalities. *)
+Module exp_Types <: SYMBOL_TYPES.
+  
+   Inductive terminal' :=
+   | Plus | Mult | LBracket | RBracket | Num
+   . 
+   
+   Definition terminal := terminal'.
+   
+   Inductive nonterminal' :=
+   | E | E' | T_ | T' | F
+   .
+   
+   Definition nonterminal := nonterminal'.
+ 
+   Lemma t_eq_dec : forall (t t' : terminal),
+	   {t = t'} + {t <> t'}.
+   Proof. decide equality. Defined.
+   
+   Lemma nt_eq_dec : forall (nt nt' : nonterminal),
+	   {nt = nt'} + {nt <> nt'}.
+   Proof. decide equality. Defined.
+ 
+   Definition showT (a : terminal) : string :=
+	 match a with
+	 | Plus    => "+"
+	 | Mult  => "*"
+	 | LBracket  => "("
+	 | RBracket => ")"
+	 | Num => "Num"
+	 end.
+ 
+   Definition showNT (x : nonterminal) : string :=
+	 match x with
+	 | E => "E"
+	 | E' => "E'"
+	 | T_ => "T"
+	 | T' => "T'"
+	 | F => "F"
+	 end.
+   
+   (* A Num token carries a natural number -- no other token
+	  carries a meaningful semantic value. *)
+   Definition t_semty (a : terminal) : Type :=
+	 match a with
+	 | Num => nat
+	 | _   => unit
+	 end.
+ 
+   Definition nt_semty (x : nonterminal) : Type :=
+	 match x with
+	 | E => exp
+	 | E' => exp'
+	 | T_ => term
+   | T' => term'
+   | F => fact
+	 end.
+ 
+ End exp_Types.
+
+
+Module Export G <: Grammar.T.
+  Module Export SymTy := exp_Types.
+  Module Export Defs  := DefsFn SymTy.
+End G.
+
+Definition exp_grammar : grammar :=
+  {| start := E ;
+     prods := [existT action_ty
+                      (E, [NT T_; NT E'])
+                      (fun tup =>
+                         match tup with
+                         | (t, (e, _)) =>
+                           comb_exp t e
+                         end);
+               existT action_ty
+                      (E', [T Plus; NT T_; NT E'])
+                      (fun tup =>
+                         match tup with
+                         | (_, (t, (e', _))) =>
+                           comb_exp' t e'
+                         end);
+               existT action_ty
+                      (E', [])
+                      (fun tup => 
+                         match tup with
+                         | _ => empty_exp'
+                         end);
+               existT action_ty
+                      (T_, [NT F; NT T'])
+                      (fun tup =>
+                         match tup with
+                         | (f, (t', _)) =>
+                           comb_term f t'
+                         end);
+               existT action_ty
+                      (T', [T Mult; NT F; NT T'])
+                      (fun tup =>
+                         match tup with
+                         | (_, (f, (t', _))) =>
+                           comb_term' f t'
+                         end);
+               existT action_ty
+                      (F, [T LBracket; NT E; T RBracket])
+                      (fun tup =>
+                         match tup with
+                         | (_, (e, (_, _))) =>
+                           exp_fact e
+                         end);
+               existT action_ty
+                      (F, [T Num])
+                      (fun tup =>
+                         match tup with
+                         | (n, _) =>
+                           num_fact n
+                         end)
+              ]
+  |}.
+
+Definition tok (a : terminal) (v : t_semty a) : token :=
+  existT _ a v.
+
+
+(**
+    Inductive nullable_sym (g : grammar) : symbol -> Prop :=
+    | NullableSym : forall x ys f,
+        In (existT _ (x, ys) f) g.(prods)
+        -> nullable_gamma g  
+        -> nullable_sym g (NT x)
+(* Note, this means, if we want to write an empty production, we need to explicitly state it as going to empty set [] *)
+(* Specification of nullable_grammar *)
+    with nullable_gamma (g : grammar) : list symbol -> Prop :=
+         | NullableNil  : nullable_gamma g [] (* rhs is blank, that's empty *)
+         | NullableCons : forall hd: symbol tl: [symbol],
+             nullable_sym g hd
+             -> nullable_gamma g tl
+             -> nullable_gamma g (hd :: tl).
+**)
+
+Theorem E'_is_nullable : forall (g: grammar) (t: terminal), nullable_sym g (NT E').
+Proof. 
+  intros.
+  apply NullableSym with (ys := []) (f := (fun tup => match tup with | _ => empty_exp' end)).
+  - simpl. repeat (try apply in_eq; try apply in_cons). (* This will navigate through the list until we find our production *)
+  - apply NullableNil.
+Qed.
+
+
+ 
+
+ 
+
+ 
+ 
+ 
+ 
+ 
+ 
+ 
